theories/Substitution/Introductions/Nat.v
@@ -1,7 +1,7 @@
 From LogRel.AutoSubst Require Import core unscoped Ast Extra.
-From LogRel Require Import Utils BasicAst Notations Context NormalForms Weakening GenericTyping LogicalRelation Validity.
-From LogRel.LogicalRelation Require Import Induction Irrelevance Escape Reflexivity Weakening Neutral Transitivity Reduction Application Universe SimpleArr.
-From LogRel.Substitution Require Import Irrelevance Properties Conversion SingleSubst Reflexivity.
+From LogRel Require Import Utils BasicAst Notations LContexts Context NormalForms Weakening GenericTyping Monad LogicalRelation Validity.
+From LogRel.LogicalRelation Require Import Induction Irrelevance Escape Reflexivity Weakening Monotonicity Split Neutral Transitivity Reduction Application Universe SimpleArr.
+From LogRel.Substitution Require Import Irrelevance Properties Conversion SingleSubst Reflexivity Monotonicity.
 From LogRel.Substitution.Introductions Require Import Universe Pi SimpleArr Var.
 
 Set Universe Polymorphism.
@@ -12,32 +12,39 @@ Context `{GenericTypingProperties}.
 Set Printing Primitive Projection Parameters.
 
 
-Lemma natRed {Γ l} : [|- Γ] -> [Γ ||-<l> tNat].
+Lemma natRed {wl Γ l} : [|- Γ]< wl > -> [Γ ||-<l> tNat]< wl >.
 Proof. 
   intros; eapply LRNat_; constructor; eapply redtywf_refl; gen_typing.
 Defined.
 
-Lemma natValid {Γ l} (VΓ : [||-v Γ]) : [Γ ||-v<l> tNat | VΓ].
+Lemma WnatRed {wl Γ l} : [|- Γ]< wl > -> W[Γ ||-<l> tNat]< wl >.
 Proof.
-  unshelve econstructor; intros.
-  + now eapply natRed.
-  + cbn; constructor; eapply redtywf_refl; gen_typing.
+  intros ; now eapply LogtoW, natRed.
 Defined.
 
-Lemma natconvValid {Γ l} (VΓ : [||-v Γ]) (VNat : [Γ ||-v<l> tNat | VΓ]) : 
-  [Γ ||-v<l> tNat ≅ tNat | VΓ | VNat].
+Lemma natValid {wl Γ l} (VΓ : [||-v Γ]< wl >) : [Γ ||-v<l> tNat | VΓ]< wl >.
 Proof.
-  constructor; intros.
-  enough [Δ ||-<l> tNat ≅ tNat | natRed wfΔ] by irrelevance.
+  unshelve econstructor; intros.
+  + now eapply WnatRed.
+  + cbn ; eapply EqLogtoW.
+    constructor; eapply redtywf_refl.
+    now gen_typing.
+Defined.
+
+Lemma natconvValid {wl Γ l} (VΓ : [||-v Γ]< wl >) (VNat : [Γ ||-v<l> tNat | VΓ]< wl >) : 
+  [Γ ||-v<l> tNat ≅ tNat | VΓ | VNat]< wl >.
+Proof.
+  constructor; intros ; cbn.
+  unshelve eapply EqLogtoW' ; [exact (natRed wfΔ) | ].
   constructor; cbn; eapply redtywf_refl; gen_typing.
 Qed.
 
-Lemma redUOne {Γ} : [|- Γ] -> [Γ ||-U<one> U].
+Lemma redUOne {wl Γ} : [|- Γ]< wl > -> [Γ ||-U<one> U]< wl >.
 Proof.
   intros ; econstructor; [easy| gen_typing|eapply redtywf_refl; gen_typing].
 Defined.
 
-Lemma natTermRed {Δ} (wfΔ : [|-Δ]) : [Δ ||-<one> tNat : U | LRU_ (redUOne wfΔ)].
+Lemma natTermRed {wl Δ} (wfΔ : [|-Δ]< wl >) : [Δ ||-<one> tNat : U | LRU_ (redUOne wfΔ)]< wl >.
 Proof.
   econstructor.
   + eapply redtmwf_refl; gen_typing.
@@ -46,39 +53,65 @@ Proof.
   + now eapply (natRed (l:= zero)).
 Defined.
 
-Lemma natTermValid {Γ} (VΓ : [||-v Γ]):  [Γ ||-v<one> tNat : U | VΓ | UValid VΓ].
+Lemma natTermValid {wl Γ} (VΓ : [||-v Γ]< wl >):  [Γ ||-v<one> tNat : U | VΓ | UValid VΓ]< wl >.
 Proof.
   constructor; intros.
-  - eapply natTermRed. 
-  - eexists (natTermRed wfΔ) (natTermRed wfΔ) (natRed wfΔ); cbn.
+  - eapply TmLogtoW' ; eapply natTermRed.
+    Unshelve. assumption.
+  - unshelve eapply TmEqLogtoW'.
+    1: cbn ; eapply LRU_ ; unshelve econstructor ; [ | now econstructor | eassumption |.. ].
+    1: eapply redtywf_refl ; gen_typing.
+    eexists (natTermRed wfΔ) (natTermRed wfΔ) (natRed wfΔ); cbn.
     + gen_typing.
     + now eapply (natRed (l:=zero)).
     + constructor; eapply redtywf_refl; gen_typing.
 Qed.
 
-Lemma zeroRed {Γ l} {NN : [Γ ||-Nat tNat]} (wfΓ : [|- Γ]): [Γ ||-<l> tZero : _ | LRNat_ l NN].
+Lemma zeroRed {wl Γ l} {NN : [Γ ||-Nat tNat]< wl >} (wfΓ : [|- Γ]< wl >): [Γ ||-<l> tZero : _ | LRNat_ l NN]< wl >.
 Proof.
   exists tZero.
   1,2: gen_typing.
   constructor.
 Defined.
 
-Lemma zeroRedEq {Γ l} {NN : [Γ ||-Nat tNat]} (wfΓ : [|- Γ]): [Γ ||-<l> tZero ≅ tZero : _ | LRNat_ l NN].
+Lemma WzeroRed {wl Γ l} {NN : [Γ ||-Nat tNat]< wl >} (wfΓ : [|- Γ]< wl >): W[Γ ||-<l> tZero : _ | LogtoW (LRNat_ l NN)]< wl >.
+Proof.
+  exists (leaf _).
+  intros wl' Ho Ho' ; pose (f := over_tree_le Ho).
+  exists tZero.
+  + eapply redtmwf_Ltrans ; [eassumption | now gen_typing].
+  + eapply convtm_Ltrans ; [eassumption | now gen_typing].
+  + constructor.
+Defined.
+
+Lemma zeroRedEq {wl Γ l} {NN : [Γ ||-Nat tNat]< wl >} (wfΓ : [|- Γ]< wl >): [Γ ||-<l> tZero ≅ tZero : _ | LRNat_ l NN]< wl >.
 Proof.
   exists tZero tZero.
   1-3: gen_typing.
   constructor.
 Defined.
 
-Lemma zeroValid {Γ l} (VΓ : [||-v Γ]): 
-  [Γ ||-v<l> tZero : tNat | VΓ | natValid VΓ].
+Lemma WzeroRedEq {wl Γ l} {NN : [Γ ||-Nat tNat]< wl >} (wfΓ : [|- Γ]< wl >):
+  W[Γ ||-<l> tZero ≅ tZero : _ | LogtoW (LRNat_ l NN)]< wl >.
 Proof.
-  constructor; intros; cbn; [unshelve eapply zeroRed| unshelve eapply zeroRedEq]; tea.
+  exists (leaf _) ; intros wl' Ho Ho' ; pose (f := over_tree_le Ho).
+  exists tZero tZero.
+  1,2: eapply redtmwf_Ltrans ; [eassumption | now gen_typing].
+  + eapply convtm_Ltrans ; [eassumption | now gen_typing].
+  + constructor.
+Defined.
+
+Lemma zeroValid {wl Γ l} (VΓ : [||-v Γ]< wl >): 
+  [Γ ||-v<l> tZero : tNat | VΓ | natValid VΓ]< wl >.
+Proof.
+  constructor; intros ; cbn.
+  + eapply TmLogtoW, zeroRed ; assumption.
+  + eapply TmEqLogtoW, zeroRedEq; tea.
 Qed.
 
-Lemma succRed {Γ l n} {NN : [Γ ||-Nat tNat]} :
-  [Γ ||-<l> n : _ | LRNat_ l NN] ->
-  [Γ ||-<l> tSucc n : _ | LRNat_ l NN].
+Lemma succRed {wl Γ l n} {NN : [Γ ||-Nat tNat]< wl >} :
+  [Γ ||-<l> n : _ | LRNat_ l NN]< wl > ->
+  [Γ ||-<l> tSucc n : _ | LRNat_ l NN]< wl >.
 Proof.
   intros Rn; exists (tSucc n).
   + eapply redtmwf_refl; eapply ty_succ; now escape.
@@ -86,11 +119,24 @@ Proof.
   + now constructor.
 Defined.
 
-Lemma succRedEq {Γ l n n'} {NN : [Γ ||-Nat tNat]} :
-  [Γ ||-<l> n : _ | LRNat_ l NN] ->
-  [Γ ||-<l> n' : _ | LRNat_ l NN] ->
-  [Γ ||-<l> n ≅ n' : _ | LRNat_ l NN] ->
-  [Γ ||-<l> tSucc n ≅ tSucc n' : _ | LRNat_ l NN].
+Lemma WsuccRed {wl Γ l n} {NN : [Γ ||-Nat tNat]< wl >} :
+  W[Γ ||-<l> n : _ | LogtoW (LRNat_ l NN) ]< wl > ->
+  W[Γ ||-<l> tSucc n : _ | LogtoW (LRNat_ l NN)]< wl >.
+Proof.
+  intros Rn ; exists (WTTm _ Rn).
+  intros wl' Ho Ho' ; exists (tSucc n).
+  + eapply redtmwf_refl; eapply ty_succ, ty_Ltrans ; [ | now Wescape].
+    now eapply over_tree_le.
+  + eapply convtm_succ; eapply escapeEqTerm, reflLRTmEq.
+    now unshelve eapply Rn.
+  + constructor ; now unshelve eapply Rn.
+Defined.
+
+Lemma succRedEq {wl Γ l n n'} {NN : [Γ ||-Nat tNat]< wl >} :
+  [Γ ||-<l> n : _ | LRNat_ l NN]< wl > ->
+  [Γ ||-<l> n' : _ | LRNat_ l NN]< wl > ->
+  [Γ ||-<l> n ≅ n' : _ | LRNat_ l NN]< wl > ->
+  [Γ ||-<l> tSucc n ≅ tSucc n' : _ | LRNat_ l NN]< wl >.
 Proof.
   intros ???; escape; exists (tSucc n) (tSucc n').
   1,2: eapply redtmwf_refl; now eapply ty_succ.
@@ -98,32 +144,48 @@ Proof.
   + now constructor.
 Defined.
 
-Lemma succRedInv {Γ l n} {NN : [Γ ||-Nat tNat]} :
-  [Γ ||-<l> tSucc n : _ | LRNat_ l NN] ->
-  [Γ ||-<l> n : _ | LRNat_ l NN].
+Lemma WsuccRedEq {wl Γ l n n'} {NN : [Γ ||-Nat tNat]< wl >} :
+  W[Γ ||-<l> n : _ | LogtoW (LRNat_ l NN)]< wl > ->
+  W[Γ ||-<l> n' : _ | LogtoW (LRNat_ l NN) ]< wl > ->
+  W[Γ ||-<l> n ≅ n' : _ | LogtoW (LRNat_ l NN)]< wl > ->
+  W[Γ ||-<l> tSucc n ≅ tSucc n' : _ | LogtoW (LRNat_ l NN)]< wl >.
+Proof.
+  intros Rn Rn' Rnn'.
+  econstructor ; intros wl' Ho Ho'.
+  pose (f:= over_tree_le Ho) ; Wescape.
+  exists (tSucc n) (tSucc n').
+  1,2: now eapply redtmwf_refl, ty_succ, ty_Ltrans.
+  - now eapply convtm_succ, convtm_Ltrans.
+  - constructor ; eapply Rnn'.
+    eassumption.
+Defined.
+
+Lemma succRedInv {wl Γ l n} {NN : [Γ ||-Nat tNat]< wl >} :
+  [Γ ||-<l> tSucc n : _ | LRNat_ l NN]< wl > ->
+  [Γ ||-<l> n : _ | LRNat_ l NN]< wl >.
 Proof.
   intros RSn; inversion RSn; subst. 
   unshelve epose proof (redtmwf_whnf red _). 1: constructor.
   subst. inversion prop; subst; tea.
-  match goal with H : [ _ ||-NeNf _ : _] |- _ => destruct H; apply convneu_whne in refl; inv_whne end.
+  match goal with H : [ _ ||-NeNf _ : _]< wl > |- _ => destruct H; apply convneu_whne in refl; inv_whne end.
 Qed.
 
-Lemma succValid {Γ l n} (VΓ : [||-v Γ]) 
-  (Vn : [Γ ||-v<l> n : tNat | VΓ | natValid VΓ]) :
-  [Γ ||-v<l> tSucc n : tNat | VΓ | natValid VΓ].
+Lemma succValid {wl Γ l n} (VΓ : [||-v Γ]< wl >) 
+  (Vn : [Γ ||-v<l> n : tNat | VΓ | natValid VΓ]< wl >) :
+  [Γ ||-v<l> tSucc n : tNat | VΓ | natValid VΓ]< wl >.
 Proof.
   constructor; intros; cbn.
-  - instValid Vσ ; now unshelve eapply succRed.
-  - instAllValid Vσ Vσ' Vσσ'; now unshelve eapply succRedEq.
+  - instValid Vσ ; now unshelve eapply WsuccRed.
+  - instAllValid Vσ Vσ' Vσσ'; now unshelve eapply WsuccRedEq.
 Qed.
 
-Lemma succcongValid {Γ l n n'} (VΓ : [||-v Γ]) 
-  (Vn : [Γ ||-v<l> n : tNat | VΓ | natValid VΓ])
-  (Vn' : [Γ ||-v<l> n' : tNat | VΓ | natValid VΓ])
-  (Veqn : [Γ ||-v<l> n ≅ n' : tNat | VΓ | natValid VΓ]) :
-  [Γ ||-v<l> tSucc n ≅ tSucc n' : tNat | VΓ | natValid VΓ].
+Lemma succcongValid {wl Γ l n n'} (VΓ : [||-v Γ]< wl >) 
+  (Vn : [Γ ||-v<l> n : tNat | VΓ | natValid VΓ]< wl >)
+  (Vn' : [Γ ||-v<l> n' : tNat | VΓ | natValid VΓ]< wl >)
+  (Veqn : [Γ ||-v<l> n ≅ n' : tNat | VΓ | natValid VΓ]< wl >) :
+  [Γ ||-v<l> tSucc n ≅ tSucc n' : tNat | VΓ | natValid VΓ]< wl >.
 Proof.
-  constructor; intros; cbn; instValid Vσ; now unshelve eapply succRedEq.
+  constructor; intros; cbn; instValid Vσ; now unshelve eapply WsuccRedEq.
 Qed.
 
 
@@ -136,10 +198,12 @@ Proof.
   now rewrite up_liftSubst_eq.
 Qed.
 
+
 Lemma liftSubst_singleSubst_eq {t u v: term} : t[u]⇑[v..] = t[u[v..]..].
 Proof. now bsimpl. Qed.
 
-Definition natElim {Γ A} (P hz hs : term) {n} {NA : [Γ ||-Nat A]} (p : NatProp NA n) : term.
+
+Definition natElim {wl Γ A} (P hz hs : term) {n} {NA : [Γ ||-Nat A]< wl >} (p : NatProp NA n) : term.
 Proof.
   destruct p.
   - exact hz.
@@ -148,40 +212,40 @@ Proof.
 Defined.
 
 Section NatElimRed.
-  Context {Γ l P hs hz}
-    (wfΓ : [|- Γ])
-    (NN : [Γ ||-Nat tNat])
-    (RN := LRNat_ _ NN)
-    (RP : [Γ,, tNat ||-<l> P])
-    (RPpt : forall n, [Γ ||-<l> n : _ | RN] -> [Γ ||-<l> P[n..]])
-    (RPext : forall n n' (Rn : [Γ ||-<l> n : _ | RN]),
-      [Γ ||-<l> n' : _ | RN] ->
-      [Γ ||-<l> n ≅ n' : _ | RN] ->
-      [Γ ||-<l> P[n..] ≅ P[n'..] | RPpt _ Rn])
+  Context {wl Γ l P hs hz}
+    (wfΓ : [|- Γ]< wl >)
+    (NN : [Γ ||-Nat tNat]< wl >)
+    (RN := (LRNat_ _ NN))
+    (RP : [Γ,, tNat ||-<l> P]< wl >)
+    (RPpt : forall n, [Γ ||-<l> n : _ | RN]< wl > -> W[Γ ||-<l> P[n..]]< wl >)
+    (RPext : forall n n' (Rn : [Γ ||-<l> n : _ | RN]< wl >),
+      [Γ ||-<l> n' : _ | RN]< wl > ->
+      [Γ ||-<l> n ≅ n' : _ | RN]< wl > ->
+      W[Γ ||-<l> P[n..] ≅ P[n'..] | RPpt _ Rn]< wl >)
     (RPz := RPpt _ (zeroRed wfΓ))
-    (Rhz : [Γ ||-<l> hz : P[tZero..] | RPz]) 
-    (RPs : [Γ ||-<l> elimSuccHypTy P])
-    (Rhs : [Γ ||-<l> hs : _ | RPs]).
+    (Rhz : W[Γ ||-<l> hz : P[tZero..] | RPz]< wl >) 
+    (RPs : W[Γ ||-<l> elimSuccHypTy P]< wl >)
+    (Rhs : W[Γ ||-<l> hs : _ | RPs]< wl >).
 
   Definition natRedElimStmt :=
-    (forall n (Rn : [Γ ||-<l> n : _ | RN]), 
-      [Γ ||-<l> tNatElim P hz hs n : _ | RPpt _ Rn ] ×
-      [Γ ||-<l> tNatElim P hz hs n ≅ tNatElim P hz hs (NatRedTm.nf Rn) : _ | RPpt _ Rn]) ×
-    (forall n (Nn : NatProp NN n) (Rn : [Γ ||-<l> n : _ | RN]), 
-      [Γ ||-<l> tNatElim P hz hs n : _ | RPpt _ Rn ] ×
-      [Γ ||-<l> tNatElim P hz hs n ≅ natElim P hz hs Nn : _ | RPpt _ Rn]).
+    (forall n (Rn : [Γ ||-<l> n : _ | RN]< wl >), 
+      W[Γ ||-<l> tNatElim P hz hs n : _ | RPpt _ Rn ]< wl > ×
+      W[Γ ||-<l> tNatElim P hz hs n ≅ tNatElim P hz hs (NatRedTm.nf Rn) : _ | RPpt _ Rn]< wl >) ×
+    (forall n (Nn : NatProp NN n) (Rn : [Γ ||-<l> n : _ | RN]< wl >), 
+      W[Γ ||-<l> tNatElim P hz hs n : _ | RPpt _ Rn ]< wl > ×
+      W[Γ ||-<l> tNatElim P hz hs n ≅ natElim P hz hs Nn : _ | RPpt _ Rn]< wl >).
 
   Lemma natElimRedAux : natRedElimStmt.
   Proof.
-    escape.
+    escape ; Wescape.
     apply NatRedInduction.
     - intros ? nf red ? nfprop ih.
-      assert [Γ ||-<l> nf : _ | RN]. 1:{
+      assert [Γ ||-<l> nf : _ | RN]< wl >. 1:{
         econstructor; tea.
         eapply redtmwf_refl; gen_typing.
       }
-      eapply redSubstTerm.
-      + eapply LRTmRedConv. 
+      eapply WredSubstTerm.
+      + eapply WLRTmRedConv. 
         2: unshelve eapply ih; tea.
         eapply RPext. 
         2: eapply LRTmEqSym.
@@ -189,107 +253,107 @@ Section NatElimRed.
       + eapply redtm_natelim; tea.
         cbn; gen_typing.
     - intros. 
-      eapply redSubstTerm.
+      eapply WredSubstTerm.
       2: eapply redtm_natElimZero; tea.
-      irrelevance.
-    - intros n Rn ih RSucc; change [Γ ||-<l> n : tNat | RN] in Rn.
-      eapply redSubstTerm.
+      Wirrelevance.
+    - intros n Rn ih RSucc; change [Γ ||-<l> n : tNat | RN]< wl > in Rn.
+      eapply WredSubstTerm.
       2: eapply redtm_natElimSucc; tea.
       2: now escape.
-      eapply simple_appTerm.
+      eapply Wsimple_appTerm.
       2: eapply ih.
-      irrelevance0.
-      2: unshelve eapply (appTerm RPs Rhs Rn).
+      Wirrelevance0.
+      2: unshelve eapply (WappTerm RPs Rhs (TmLogtoW _ Rn)).
       now bsimpl.
     - intros ? [] ?.
-      apply reflect.
-      + apply completeness.
+      eapply Wreflect.
+      + apply Wcompleteness.
       + now eapply ty_natElim.
       + now eapply ty_natElim.
       + eapply convneu_natElim; tea.
         { eapply escapeEq, reflLRTyEq. }
-        { eapply escapeEqTerm; now eapply reflLRTmEq. }
-        { eapply escapeEqTerm; now eapply reflLRTmEq. }
+        { now eapply WescapeEqTerm, WreflLRTmEq. }
+        { eapply WescapeEqTerm; now eapply WreflLRTmEq. }
     Unshelve.
-    * eapply ArrRedTy; now eapply RPpt.
-    * rewrite subst_arr. eapply ArrRedTy.
+    * eapply WArrRedTy; now eapply RPpt.
+    * rewrite subst_arr. eapply WArrRedTy.
       2: rewrite liftSubst_singleSubst_eq; cbn.
       all: now eapply RPpt.
     * exact l.
     * assumption.
   Qed.
 
-  Lemma natElimRed : forall n (Rn : [Γ ||-<l> n : _ | RN]), [Γ ||-<l> tNatElim P hz hs n : _ | RPpt _ Rn ].
+  Lemma natElimRed : forall n (Rn : [Γ ||-<l> n : _ | RN]< wl >), W[Γ ||-<l> tNatElim P hz hs n : _ | RPpt _ Rn ]< wl >.
   Proof. intros. apply (fst natElimRedAux). Qed.
 End NatElimRed.
 
 
 Section NatElimRedEq.
-  Context {Γ l P Q hs hs' hz hz'}
-    (wfΓ : [|- Γ])
-    (NN : [Γ ||-Nat tNat])
+  Context {wl Γ l P Q hs hs' hz hz'}
+    (wfΓ : [|- Γ]< wl >)
+    (NN : [Γ ||-Nat tNat]< wl >)
     (RN := LRNat_ _ NN)
-    (RP : [Γ,, tNat ||-<l> P])
-    (RQ : [Γ,, tNat ||-<l> Q])
-    (eqPQ : [Γ,, tNat |- P ≅ Q])
-    (RPpt : forall n, [Γ ||-<l> n : _ | RN] -> [Γ ||-<l> P[n..]])
-    (RQpt : forall n, [Γ ||-<l> n : _ | RN] -> [Γ ||-<l> Q[n..]])
-    (RPQext : forall n n' (Rn : [Γ ||-<l> n : _ | RN]),
-      [Γ ||-<l> n' : _ | RN] ->
-      [Γ ||-<l> n ≅ n' : _ | RN] ->
-      [Γ ||-<l> P[n..] ≅ Q[n'..] | RPpt _ Rn])
+    (RP : [Γ,, tNat ||-<l> P]< wl >)
+    (RQ : [Γ,, tNat ||-<l> Q]< wl >)
+    (eqPQ : [Γ,, tNat |- P ≅ Q]< wl >)
+    (RPpt : forall n, [Γ ||-<l> n : _ | RN]< wl > -> W[Γ ||-<l> P[n..]]< wl >)
+    (RQpt : forall n, [Γ ||-<l> n : _ | RN]< wl > -> W[Γ ||-<l> Q[n..]]< wl >)
+    (RPQext : forall n n' (Rn : [Γ ||-<l> n : _ | RN]< wl >),
+      [Γ ||-<l> n' : _ | RN]< wl > ->
+      [Γ ||-<l> n ≅ n' : _ | RN]< wl > ->
+      W[Γ ||-<l> P[n..] ≅ Q[n'..] | RPpt _ Rn]< wl >)
     (RPz := RPpt _ (zeroRed wfΓ))
     (RQz := RQpt _ (zeroRed wfΓ))
-    (Rhz : [Γ ||-<l> hz : P[tZero..] | RPz]) 
-    (RQhz : [Γ ||-<l> hz' : Q[tZero..] | RQz]) 
-    (RPQhz : [Γ ||-<l> hz ≅ hz' : _ | RPz])
-    (RPs : [Γ ||-<l> elimSuccHypTy P])
-    (RQs : [Γ ||-<l> elimSuccHypTy Q])
-    (Rhs : [Γ ||-<l> hs : _ | RPs])
-    (RQhs : [Γ ||-<l> hs' : _ | RQs])
-    (RPQhs : [Γ ||-<l> hs ≅ hs' : _ | RPs ])
+    (Rhz : W[Γ ||-<l> hz : P[tZero..] | RPz]< wl >) 
+    (RQhz : W[Γ ||-<l> hz' : Q[tZero..] | RQz]< wl >) 
+    (RPQhz : W[Γ ||-<l> hz ≅ hz' : _ | RPz]< wl >)
+    (RPs : W[Γ ||-<l> elimSuccHypTy P]< wl >)
+    (RQs : W[Γ ||-<l> elimSuccHypTy Q]< wl >)
+    (Rhs : W[Γ ||-<l> hs : _ | RPs]< wl >)
+    (RQhs : W[Γ ||-<l> hs' : _ | RQs]< wl >)
+    (RPQhs : W[Γ ||-<l> hs ≅ hs' : _ | RPs ]< wl >)
     .
 
-  Lemma RPext : forall n n' (Rn : [Γ ||-<l> n : _ | RN]),
-      [Γ ||-<l> n' : _ | RN] ->
-      [Γ ||-<l> n ≅ n' : _ | RN] ->
-      [Γ ||-<l> P[n..] ≅ P[n'..] | RPpt _ Rn].
+  Lemma RPext : forall n n' (Rn : [Γ ||-<l> n : _ | RN]< wl >),
+      [Γ ||-<l> n' : _ | RN]< wl > ->
+      [Γ ||-<l> n ≅ n' : _ | RN]< wl > ->
+      W[Γ ||-<l> P[n..] ≅ P[n'..] | RPpt _ Rn]< wl >.
   Proof.
-    intros. eapply transEq; [| eapply LRTyEqSym ]; eapply RPQext; cycle 1; tea.
+    intros. eapply WtransEq; [| eapply WLRTyEqSym ]; eapply RPQext; cycle 1; tea.
     now eapply reflLRTmEq.
     Unshelve. 2,3: eauto.
   Qed.
 
-  Lemma natElimRedAuxLeft : @natRedElimStmt _ _ P hs hz NN RPpt.
+  Lemma natElimRedAuxLeft : @natRedElimStmt _ _ _ P hs hz NN RPpt.
   Proof.
     eapply natElimRedAux; tea.
     + eapply RPext.
   Qed.
 
-  Lemma natElimRedAuxRight : @natRedElimStmt _ _ Q hs' hz' NN RQpt.
+  Lemma natElimRedAuxRight : @natRedElimStmt _ _ _ Q hs' hz' NN RQpt.
   Proof.
     eapply natElimRedAux; tea.
-    + intros. eapply transEq; [eapply LRTyEqSym |]; eapply RPQext; cycle 1; tea.
+    + intros. eapply WtransEq; [eapply WLRTyEqSym |]; eapply RPQext; cycle 1; tea.
       now eapply reflLRTmEq.
     Unshelve. all:tea.
   Qed.
 
   Lemma natElimRedEqAux :
-    (forall n n' (Rnn' : [Γ ||-<l> n ≅ n' : _ | RN]) (Rn : [Γ ||-<l> n : _ | RN]) (Rn' : [Γ ||-<l> n' : _ | RN]), 
-      [Γ ||-<l> tNatElim P hz hs n ≅ tNatElim Q hz' hs' n' : _ | RPpt _ Rn ]) ×
-    (forall n n' (Rnn' : NatPropEq NN n n') (Rn : [Γ ||-<l> n : _ | RN]) (Rn' : [Γ ||-<l> n' : _ | RN]), 
-      [Γ ||-<l> tNatElim P hz hs n ≅ tNatElim Q hz' hs' n' : _ | RPpt _ Rn ]).
+    (forall n n' (Rnn' : [Γ ||-<l> n ≅ n' : _ | RN]< wl >) (Rn : [Γ ||-<l> n : _ | RN]< wl >) (Rn' : [Γ ||-<l> n' : _ | RN]< wl >), 
+      W[Γ ||-<l> tNatElim P hz hs n ≅ tNatElim Q hz' hs' n' : _ | RPpt _ Rn ]< wl >) ×
+    (forall n n' (Rnn' : NatPropEq NN n n') (Rn : [Γ ||-<l> n : _ | RN]< wl >) (Rn' : [Γ ||-<l> n' : _ | RN]< wl >), 
+      W[Γ ||-<l> tNatElim P hz hs n ≅ tNatElim Q hz' hs' n' : _ | RPpt _ Rn ]< wl >).
   Proof.
     apply NatRedEqInduction.
-    - intros ?? nfL nfR redL redR ? prop ih RL RR; destruct (NatPropEq_whnf prop).
-      assert [Γ ||-<l> nfL : _ | RN] by (eapply redTmFwd; cycle 1; tea).
-      assert [Γ ||-<l> nfR : _ | RN] by (eapply redTmFwd; cycle 1; tea).
-      eapply LREqTermHelper.
+    - intros ?? nfL nfR redL redR ? prop ih RL RR ; destruct (NatPropEq_whnf prop).
+      assert [Γ ||-<l> nfL : _ | RN]< wl > by (eapply redTmFwd; cycle 1; tea).
+      assert [Γ ||-<l> nfR : _ | RN]< wl > by (eapply redTmFwd; cycle 1; tea).
+      eapply WLREqTermHelper.
       * eapply (fst natElimRedAuxLeft).
       * eapply (fst natElimRedAuxRight).
       * eapply RPQext. 1: tea.
         now econstructor.
-      * eapply LRTmEqRedConv.
+      * eapply WLRTmEqRedConv.
         + eapply RPext; tea. 
           eapply LRTmEqSym; eapply redwfSubstTerm; cycle 1; tea.
         + unshelve erewrite (redtmwf_det _ _ (NatRedTm.red RL) redL); tea.
@@ -298,38 +362,40 @@ Section NatElimRedEq.
           1: dependent inversion RR; subst; cbn; now eapply NatProp_whnf.
           now eapply ih.
         Unshelve. tea.
-    - intros. eapply LREqTermHelper.
+    - intros. eapply WLREqTermHelper.
       * unshelve eapply (snd natElimRedAuxLeft); constructor.
       * unshelve eapply (snd natElimRedAuxRight); tea; constructor.
       * eapply RPQext; [unshelve eapply zeroRed| unshelve eapply zeroRedEq]; tea.
-      * cbn; irrelevance.
+      * cbn; Wirrelevance.
     - intros ??? ih Rn Rn'. pose proof (succRedInv Rn); pose proof (succRedInv Rn').
-      eapply LREqTermHelper.
+      eapply WLREqTermHelper.
       * unshelve eapply (snd natElimRedAuxLeft); now constructor.
       * unshelve eapply (snd natElimRedAuxRight); tea; now constructor.
       * eapply RPQext; [unshelve eapply succRed| unshelve eapply succRedEq]; tea.
       * cbn.
-        eapply simple_appcongTerm.
+        eapply Wsimple_appcongTerm.
         4: now eapply ih.
-        + irrelevance0. 2: eapply appcongTerm; tea.
+        + Wirrelevance0. 2: eapply WappcongTerm; tea.
           now bsimpl.
+          1,2: eapply TmLogtoW ; eassumption.
+          now eapply TmEqLogtoW.
         + eapply (fst natElimRedAuxLeft).
-        + eapply LRTmRedConv. 2: eapply (fst natElimRedAuxRight).
-          eapply LRTyEqSym; now eapply RPQext.
+        + eapply WLRTmRedConv. 2: eapply (fst natElimRedAuxRight).
+          eapply WLRTyEqSym; now eapply RPQext.
         Unshelve. 2,4,5: tea.
-        1: eapply ArrRedTy; now eapply RPpt.
-        rewrite subst_arr. eapply ArrRedTy.
+        1: eapply WArrRedTy; now eapply RPpt.
+        rewrite subst_arr. eapply WArrRedTy.
         2: rewrite liftSubst_singleSubst_eq; cbn.
         all: now eapply RPpt.
-    - intros ?? neueq ??. escape. inversion neueq.
-      assert [Γ |- P[ne..] ≅ Q[ne'..]]. 1:{
-        eapply escapeEq. eapply RPQext; tea.
+    - intros ?? neueq ??. escape ; Wescape. inversion neueq.
+      assert [Γ |- P[ne..] ≅ Q[ne'..]]< wl >. 1:{
+        eapply WescapeEq. eapply RPQext; tea.
         econstructor.
         1,2: now eapply redtmwf_refl.
         2: now constructor.
         gen_typing.
       }
-      eapply neuTermEq.
+      eapply WneuTermEq.
       + eapply ty_natElim; tea.
       + eapply ty_conv. 
         1: eapply ty_natElim; tea.
@@ -339,22 +405,22 @@ Section NatElimRedEq.
   Qed.
 
   Lemma natElimRedEq :
-    (forall n n' (Rnn' : [Γ ||-<l> n ≅ n' : _ | RN]) (Rn : [Γ ||-<l> n : _ | RN]) (Rn' : [Γ ||-<l> n' : _ | RN]), 
-      [Γ ||-<l> tNatElim P hz hs n ≅ tNatElim Q hz' hs' n' : _ | RPpt _ Rn ]).
+    (forall n n' (Rnn' : [Γ ||-<l> n ≅ n' : _ | RN]< wl >) (Rn : [Γ ||-<l> n : _ | RN]< wl >) (Rn' : [Γ ||-<l> n' : _ | RN]< wl >), 
+      W[Γ ||-<l> tNatElim P hz hs n ≅ tNatElim Q hz' hs' n' : _ | RPpt _ Rn ]< wl >).
   Proof. apply natElimRedEqAux. Qed.
 End NatElimRedEq.
 
 
 
 Section NatElimValid.
-  Context {Γ l P}
-    (VΓ : [||-v Γ])
+  Context {wl Γ l P}
+    (VΓ : [||-v Γ]< wl >)
     (VN := natValid (l:=l) VΓ)
-    (VΓN := validSnoc VΓ VN)
-    (VP : [Γ ,, tNat ||-v<l> P | VΓN]).
+    (VΓN := validSnoc' VΓ VN)
+    (VP : [Γ ,, tNat ||-v<l> P | VΓN]< wl >).
   
   Lemma elimSuccHypTyValid :
-    [Γ ||-v<l> elimSuccHypTy P | VΓ].
+    [Γ ||-v<l> elimSuccHypTy P | VΓ]< wl >.
   Proof.
     unfold elimSuccHypTy.
     unshelve eapply PiValid.
@@ -371,181 +437,340 @@ Section NatElimValid.
 
   Context {hz hs}
     (VPz := substS VP (zeroValid VΓ))
-    (Vhz : [Γ ||-v<l> hz : P[tZero..] | VΓ | VPz]) 
-    (Vhs : [Γ ||-v<l> hs : _ | VΓ | elimSuccHypTyValid]).
-
+    (Vhz : [Γ ||-v<l> hz : P[tZero..] | VΓ | VPz]< wl >) 
+    (Vhs : [Γ ||-v<l> hs : _ | VΓ | elimSuccHypTyValid]< wl >).
+Axiom todo: False.
 
   Lemma natElimValid {n}
-    (Vn : [Γ ||-v<l> n : tNat | VΓ | VN])
+    (Vn : [Γ ||-v<l> n : tNat | VΓ | VN]< wl >)
     (VPn := substS VP Vn)
-    : [Γ ||-v<l> tNatElim P hz hs n : _ | VΓ | VPn].
+    : [Γ ||-v<l> tNatElim P hz hs n : _ | VΓ | VPn]< wl >.
   Proof.
     constructor; intros.
     - instValid Vσ; cbn.
-      irrelevance0.  1: now rewrite singleSubstComm'.
       epose proof (Vuσ := liftSubstS' VN Vσ).
-      instValid Vuσ; escape.
+      unshelve eapply TreeTmSplit ; [eapply DTree_fusion ; [eapply DTree_fusion | ] ; shelve | ].
+      intros wl'' Ho HA.
+      pose (f':= over_tree_le Ho).
+      Wirrelevance0.  1: now rewrite singleSubstComm'.
+      instValid Vuσ; escape ; Wescape.
       unshelve eapply natElimRed; tea.
+      + econstructor ; eapply redtywf_refl, wft_term.
+        now eapply ty_nat, wfc_Ltrans.
       + intros m Rm.
-        rewrite up_single_subst. 
-        unshelve eapply validTy; cycle 1; tea.
-        unshelve econstructor; [now bsimpl| now cbn].
-      + rewrite elimSuccHypTy_subst. eapply validTy; tea; eapply elimSuccHypTyValid.
-      + intros m m' Rm Rm' Rmm'; cbn.
-        irrelevance0. 1: now rewrite up_single_subst.
         rewrite up_single_subst.
-        unshelve eapply validTyExt; cycle 1 ; tea.
-        1,2: unshelve econstructor; [now bsimpl| now cbn].
-        unshelve econstructor; [|now cbn].
-        bsimpl; cbn; eapply reflSubst.
-      + irrelevance.
-      + irrelevance. now rewrite elimSuccHypTy_subst. 
+        unshelve eapply validTy.
+        6: eassumption.
+        * now eapply wfLCon_le_trans.
+        * now eapply wfc_Ltrans.
+        * unshelve econstructor ; [ | now eapply TmLogtoW].
+          now bsimpl ; unshelve eapply subst_Ltrans.
+      + cbn.
+        set (Help := {|  NatRedTy.red := redtywf_refl (wft_term (ty_nat (wfc_Ltrans f' wfΔ))) |}).
+        change [Δ ||-< l > n[σ] : tNat | LRNat_ _ Help ]< wl'' >.
+        irrelevanceRefl.
+        unshelve eapply RVn.
+        1: eapply over_tree_fusion_r, over_tree_fusion_l ; exact Ho.
+        eapply over_tree_fusion_r ; exact Ho.
+      + now eapply wfc_Ltrans.
+      + rewrite elimSuccHypTy_subst.
+        unshelve eapply validTy ;[ .. | eapply elimSuccHypTyValid | ].
+        3: unshelve eapply subst_Ltrans ; cycle 1 ; eassumption.
+        now eapply wfc_Ltrans.
+      + eapply RVP ; do 2 eapply (over_tree_fusion_l).
+        exact Ho.
+      + intros m m' Rm Rm' Rmm'; cbn.
+        Wirrelevance0. 1: now rewrite up_single_subst.
+        rewrite up_single_subst.
+        unshelve eapply validTyExt ; cycle 2 ; tea.
+        1: now eapply wfLCon_le_trans.
+        1: now eapply wfc_Ltrans.
+        1,2: unshelve econstructor; [bsimpl ; now unshelve eapply subst_Ltrans| cbn].
+        1,2: now eapply TmLogtoW.
+        unshelve econstructor; [ | cbn].
+        * fsimpl; cbn; now unshelve eapply reflSubst.
+        * now eapply TmEqLogtoW.
+      + Wirrelevance0.
+        2: eapply WTm_Ltrans ; eassumption.
+        now bsimpl.
+      + Wirrelevance0.
+        2: eapply WTm_Ltrans ; eassumption.
+        now rewrite elimSuccHypTy_subst.
+        Unshelve.
+        all: eassumption.
     - instAllValid Vσ Vσ' Vσσ'.
-      irrelevance0.  1: now rewrite singleSubstComm'.
       pose (Vuσ := liftSubstS' VN Vσ).
       pose proof (Vuσ' := liftSubstS' VN Vσ').
       pose proof (Vuσrea :=  liftSubstSrealign' VN Vσσ' Vσ').
       pose proof (Vuσσ' := liftSubstSEq' VN Vσσ').
-      instValid Vuσ'; instAllValid Vuσ Vuσrea Vuσσ'; escape.
-      unshelve eapply natElimRedEq; tea; fold subst_term.
-      6-11: irrelevance; now rewrite elimSuccHypTy_subst.
-      3,4: rewrite elimSuccHypTy_subst; eapply validTy; tea; eapply elimSuccHypTyValid.
+      instValid Vuσ'; instAllValid Vuσ Vuσrea Vuσσ'; escape ; Wescape.
+      unshelve eapply TreeTmEqSplit ; [do 3 (eapply DTree_fusion) ; shelve | ].
+      intros wl'' Ho HA.
+      pose (f':= over_tree_le Ho).
+      Wirrelevance0.  1: now rewrite singleSubstComm'.
+      unshelve eapply natElimRedEq ; tea; fold subst_term.
+      15,16: Wirrelevance0 ; [ now rewrite elimSuccHypTy_subst | unshelve eapply WTm_Ltrans ; cycle 3 ; eassumption].
+      15: Wirrelevance0 ; [ now rewrite elimSuccHypTy_subst | unshelve eapply WTmEq_Ltrans ; cycle 3 ; eassumption].
+      12,13: Wirrelevance0 ; [ | unshelve eapply WTm_Ltrans ; cycle 3 ; eassumption] ; now bsimpl.
+      12: Wirrelevance0 ; [ | unshelve eapply WTmEq_Ltrans ; cycle 3 ; eassumption] ; now bsimpl.
+      6,7: rewrite elimSuccHypTy_subst; unshelve eapply validTy ; [.. | unshelve eapply elimSuccHypTyValid | ].
+      8,11: unshelve eapply subst_Ltrans ; [ .. | eassumption | | eassumption].
+      4,6,7: now eapply wfc_Ltrans.
+      + econstructor ; eapply redtywf_refl, wft_term.
+        now eapply ty_nat, wfc_Ltrans.
       + intros m Rm.
         rewrite up_single_subst. 
-        unshelve eapply validTy; cycle 1; tea.
-        unshelve econstructor; [now bsimpl| now cbn].
-      + intros m Rm.
+        unshelve eapply validTy; cycle 4; tea.
+        2: unshelve econstructor; [| now eapply TmLogtoW].
+        1: unshelve eapply subst_Ltrans ; [ .. | eassumption | | eassumption].
+      + cbn.
+        set (Help := {| NatRedTy.red := _ |}).
+        change [Δ ||-< l > n[σ] : tNat | LRNat_ _ Help ]< wl'' >.
+        irrelevanceRefl.
+        unshelve eapply RVn.
+        1: eapply over_tree_fusion_r, over_tree_fusion_l, over_tree_fusion_r ; exact Ho.
+        eapply over_tree_fusion_l, over_tree_fusion_r, over_tree_fusion_l ; exact Ho.
+      + cbn. intros m Rm.
         rewrite up_single_subst. 
-        unshelve eapply validTy; cycle 1; tea.
-        unshelve econstructor; [now bsimpl| now cbn].
+        unshelve eapply validTy; cycle 4; tea.
+        2: unshelve econstructor; [| now eapply TmLogtoW].
+        1: unshelve eapply subst_Ltrans ; [ .. | eassumption | | eassumption].
+      + unshelve eapply validTy ; cycle 4; tea.
+        do 3 eapply (over_tree_fusion_l) ; exact Ho.
+      + unshelve eapply validTy ; cycle 4; tea.
+        eapply over_tree_fusion_r  ; do 2 eapply (over_tree_fusion_l); exact Ho.
+      + now eapply convty_Ltrans.
       + intros m m' Rm Rm' Rmm'; cbn.
-        irrelevance0. 1: now rewrite up_single_subst.
+        Wirrelevance0. 1: now rewrite up_single_subst.
         rewrite up_single_subst.
-        unshelve eapply validTyExt; cycle 1 ; tea.
-        1,2: unshelve econstructor; [now bsimpl| now cbn].
-        unshelve econstructor; [|now cbn].
-        now bsimpl.
-  Qed.
+        unshelve eapply validTyExt ; cycle 3 ; tea.
+        2: now eapply wfc_Ltrans.
+        2,3: unshelve econstructor; [| now eapply TmLogtoW].
+        2,3: unshelve eapply subst_Ltrans ; [ .. | eassumption] ; eassumption.
+        unshelve econstructor; [|now eapply TmEqLogtoW].
+        bsimpl.
+        now unshelve eapply eqsubst_Ltrans.
+      + cbn.
+        set (Help := {| NatRedTy.red := _ |}).
+        change [Δ ||-< l > n[σ] ≅ n[σ'] : tNat | LRNat_ _ Help ]< wl'' >.
+        irrelevanceRefl.
+        unshelve eapply REVn.
+        1: eapply over_tree_fusion_r, over_tree_fusion_l, over_tree_fusion_r ; exact Ho.
+        do 2 eapply over_tree_fusion_r ; eapply over_tree_fusion_l ; exact Ho.
+      + cbn.
+        set (Help := {| NatRedTy.red := _ |}).
+        change [Δ ||-< l > n[σ'] : tNat | LRNat_ _ Help ]< wl'' >.
+        irrelevanceRefl.
+        unshelve eapply RVn0.
+        1: eapply over_tree_fusion_r, over_tree_fusion_l, over_tree_fusion_r ; exact Ho.
+        1: eapply over_tree_fusion_l, over_tree_fusion_l, over_tree_fusion_r ; exact Ho.
+        Unshelve. all: now constructor.
+Qed.    
 
   Lemma natElimZeroValid  : 
-    [Γ ||-v<l> tNatElim P hz hs tZero ≅ hz : _ | VΓ | VPz].
+    [Γ ||-v<l> tNatElim P hz hs tZero ≅ hz : _ | VΓ | VPz]< wl >.
   Proof.
     constructor; intros.
     epose proof (Vuσ := liftSubstS' VN Vσ).
-    instValid Vσ; instValid Vuσ; escape.
-    irrelevance0.  1: now rewrite singleSubstComm'.
+    instValid Vσ; instValid Vuσ; escape ; Wescape.
+    unshelve eapply TreeTmEqSplit ; [eapply DTree_fusion ; [eapply DTree_fusion | ] ; shelve | ].
+    intros wl'' Ho HA.
+    pose (f':= over_tree_le Ho).
+    Wirrelevance0.  1: now rewrite singleSubstComm'.
     unshelve eapply (snd (natElimRedAux _ _ _ _ _ _ _ _) _ NatRedTm.zeroR); tea; fold subst_term.
-    7: eapply zeroValid.
+    2: econstructor ; eapply  (redtywf_refl (wft_term (ty_nat (wfc_Ltrans f' wfΔ)))).
+    1: now eapply wfc_Ltrans.
+    7: irrelevanceRefl ; eapply (WRedTm _ (validTm (zeroValid _) _ _ Vσ)).
+    1: unshelve eapply (WRed _ (validTy VP _ _ Vuσ)).
+    1: eapply over_tree_fusion_l, over_tree_fusion_l ; exact Ho.
     + intros m Rm.
       rewrite up_single_subst. 
-      unshelve eapply validTy; cycle 1; tea.
-      unshelve econstructor; [now bsimpl| now cbn].
+      unshelve eapply validTy ; cycle 5 ; tea.
+      3: now eapply wfc_Ltrans.
+      unshelve econstructor; [now eapply subst_Ltrans | ].
+      now eapply TmLogtoW.
     + intros m m' Rm Rm' Rmm'; cbn.
-      irrelevance0. 1: now rewrite up_single_subst.
+      Wirrelevance0. 1: now rewrite up_single_subst.
       rewrite up_single_subst.
-      unshelve eapply validTyExt; cycle 1 ; tea.
-      1,2: unshelve econstructor; [now bsimpl| now cbn].
-      unshelve econstructor; [|now cbn].
+      unshelve eapply validTyExt ; cycle 3.
+      1: eassumption.
+      3: unshelve econstructor; [now eapply subst_Ltrans | now eapply TmLogtoW].
+      1: unshelve econstructor; [now eapply subst_Ltrans | now eapply TmLogtoW].
+      unshelve econstructor; [eapply eqsubst_Ltrans | now eapply TmEqLogtoW].
       bsimpl; cbn; eapply reflSubst.
-    + irrelevance.
-    + rewrite elimSuccHypTy_subst. eapply validTy; tea; eapply elimSuccHypTyValid.
-    + irrelevance. now rewrite elimSuccHypTy_subst. 
-    Unshelve. 4: tea.
+    + Wirrelevance0.
+      2: eapply WTm_Ltrans.
+      2: now eapply RVhz.
+      now bsimpl.
+    + rewrite elimSuccHypTy_subst. unshelve eapply validTy.
+      6: eapply elimSuccHypTyValid.
+      3: now eapply subst_Ltrans ; eassumption.
+      now eapply wfc_Ltrans.
+    + Wirrelevance0.
+      now rewrite elimSuccHypTy_subst.
+      eapply WTm_Ltrans.
+      eauto.
+      Unshelve.
+      3,5-9: eassumption.
+      3: now eapply over_tree_fusion_r, over_tree_fusion_l ; exact Ho.
+      shelve.
+    + now eapply over_tree_fusion_r ; exact Ho.
   Qed.
 
   Lemma natElimSuccValid {n}
-    (Vn : [Γ ||-v<l> n : tNat | VΓ | VN]) 
+    (Vn : [Γ ||-v<l> n : tNat | VΓ | VN]< wl >) 
     (VPSn := substS VP (succValid _ Vn)) : 
-    [Γ ||-v<l> tNatElim P hz hs (tSucc n) ≅ tApp (tApp hs n) (tNatElim P hz hs n) : _ | VΓ | VPSn].
+    [Γ ||-v<l> tNatElim P hz hs (tSucc n) ≅ tApp (tApp hs n) (tNatElim P hz hs n) : _ | VΓ | VPSn]< wl >.
   Proof.
     constructor; intros.
     epose proof (Vuσ := liftSubstS' VN Vσ).
     instValid Vσ; instValid Vuσ; escape.
-    irrelevance0.  1: now rewrite singleSubstComm'.
-    pose (NSn := NatRedTm.succR RVn).
+    unshelve eapply TreeTmEqSplit ; [do 2 eapply DTree_fusion ; shelve | ].
+    intros wl'' Ho HA.
+    pose (f':= over_tree_le Ho).
+    Wirrelevance0.  1: now rewrite singleSubstComm'.
+    pose (Ho1 := over_tree_fusion_l (over_tree_fusion_l Ho)).
+    pose (Ho2 := over_tree_fusion_r (over_tree_fusion_l Ho)).
+    epose (NSn := NatRedTm.succR (WRedTm _ RVn _ Ho1 Ho2)).
     unshelve eapply (snd (natElimRedAux _ _ _ _ _ _ _ _) _ NSn); tea; fold subst_term.
+    1: now eapply wfc_Ltrans.
+    1: unshelve eapply (WRed _ (validTy VP _ _ Vuσ)).
+    1: now eapply (over_tree_fusion_l (over_tree_fusion_r Ho)).
     + intros m Rm.
       rewrite up_single_subst. 
-      unshelve eapply validTy; cycle 1; tea.
-      unshelve econstructor; [now bsimpl| now cbn].
+      unshelve eapply validTy; cycle 4 ; tea.
+      1: now eapply wfc_Ltrans.
+      unshelve econstructor; [now eapply subst_Ltrans| cbn].
+      Wirrelevance0 ; [ reflexivity | now eapply TmLogtoW ; exact Rm].
     + intros m m' Rm Rm' Rmm'; cbn.
-      irrelevance0. 1: now rewrite up_single_subst.
+      Wirrelevance0. 1: now rewrite up_single_subst.
       rewrite up_single_subst.
-      unshelve eapply validTyExt; cycle 1 ; tea.
-      1,2: unshelve econstructor; [now bsimpl| now cbn].
-      unshelve econstructor; [|now cbn].
-      bsimpl; cbn; eapply reflSubst.
-    + irrelevance.
-    + rewrite elimSuccHypTy_subst. eapply validTy; tea; eapply elimSuccHypTyValid.
-    + irrelevance. now rewrite elimSuccHypTy_subst. 
-    + now eapply succRed.
+      unshelve eapply validTyExt; cycle 3 ; tea ; cycle 1.
+      1: now eapply wfc_Ltrans.
+      1,2: unshelve econstructor; [now eapply subst_Ltrans| cbn].
+      1,2: Wirrelevance0 ; [reflexivity | now eapply TmLogtoW].
+      unshelve econstructor; [eapply eqsubst_Ltrans |].
+      1: bsimpl; cbn; now eapply reflSubst.
+      Wirrelevance0 ; [reflexivity | now eapply TmEqLogtoW].
+    + Wirrelevance0.
+      2: eapply WTm_Ltrans.
+      2: now eapply RVhz.
+      now bsimpl.
+    + rewrite elimSuccHypTy_subst.
+      unshelve eapply validTy.
+      6: eapply elimSuccHypTyValid.
+      3: now eapply subst_Ltrans ; eassumption.
+      now eapply wfc_Ltrans.
+    + Wirrelevance0.
+      2: eapply WTm_Ltrans.
+      2: now eapply RVhs.
+       now rewrite elimSuccHypTy_subst. 
+    + eapply succRed ; cbn in *.
+      unshelve eapply (WRedTm _ RVn).
+      now eapply over_tree_fusion_r, over_tree_fusion_r, Ho.
+      Unshelve.
+      all: assumption.
   Qed.
 
 End NatElimValid.
 
-Lemma natElimCongValid {Γ l P Q hz hz' hs hs' n n'}
-    (VΓ : [||-v Γ])
+Lemma natElimCongValid {wl Γ l P Q hz hz' hs hs' n n'}
+    (VΓ : [||-v Γ]< wl >)
     (VN := natValid (l:=l) VΓ)
-    (VΓN := validSnoc VΓ VN)
-    (VP : [Γ ,, tNat ||-v<l> P | VΓN])
-    (VQ : [Γ ,, tNat ||-v<l> Q | VΓN])
-    (VPQ : [Γ ,, tNat ||-v<l> P ≅ Q | VΓN | VP])
+    (VΓN := validSnoc' VΓ VN)
+    (VP : [Γ ,, tNat ||-v<l> P | VΓN]< wl >)
+    (VQ : [Γ ,, tNat ||-v<l> Q | VΓN]< wl >)
+    (VPQ : [Γ ,, tNat ||-v<l> P ≅ Q | VΓN | VP]< wl >)
     (VPz := substS VP (zeroValid VΓ))
     (VQz := substS VQ (zeroValid VΓ))
-    (Vhz : [Γ ||-v<l> hz : P[tZero..] | VΓ | VPz]) 
-    (Vhz' : [Γ ||-v<l> hz' : Q[tZero..] | VΓ | VQz])
-    (Vheqz : [Γ ||-v<l> hz ≅ hz' : P[tZero..] | VΓ | VPz])
+    (Vhz : [Γ ||-v<l> hz : P[tZero..] | VΓ | VPz]< wl >) 
+    (Vhz' : [Γ ||-v<l> hz' : Q[tZero..] | VΓ | VQz]< wl >)
+    (Vheqz : [Γ ||-v<l> hz ≅ hz' : P[tZero..] | VΓ | VPz]< wl >)
     (VPs := elimSuccHypTyValid VΓ VP)
     (VQs := elimSuccHypTyValid VΓ VQ)
-    (Vhs : [Γ ||-v<l> hs : _ | VΓ | VPs]) 
-    (Vhs' : [Γ ||-v<l> hs' : _ | VΓ | VQs])
-    (Vheqs : [Γ ||-v<l> hs ≅ hs' : _ | VΓ | VPs]) 
-    (Vn : [Γ ||-v<l> n : _ | VΓ | VN])
-    (Vn' : [Γ ||-v<l> n' : _ | VΓ | VN])
-    (Veqn : [Γ ||-v<l> n ≅ n' : _ | VΓ | VN])
+    (Vhs : [Γ ||-v<l> hs : _ | VΓ | VPs]< wl >) 
+    (Vhs' : [Γ ||-v<l> hs' : _ | VΓ | VQs]< wl >)
+    (Vheqs : [Γ ||-v<l> hs ≅ hs' : _ | VΓ | VPs]< wl >) 
+    (Vn : [Γ ||-v<l> n : _ | VΓ | VN]< wl >)
+    (Vn' : [Γ ||-v<l> n' : _ | VΓ | VN]< wl >)
+    (Veqn : [Γ ||-v<l> n ≅ n' : _ | VΓ | VN]< wl >)
     (VPn := substS VP Vn) :
-    [Γ ||-v<l> tNatElim P hz hs n ≅ tNatElim Q hz' hs' n' : _ | VΓ | VPn].
+    [Γ ||-v<l> tNatElim P hz hs n ≅ tNatElim Q hz' hs' n' : _ | VΓ | VPn]< wl >.
 Proof.
   constructor; intros.
   pose (Vuσ := liftSubstS' VN Vσ).
-  instValid Vσ; instValid Vuσ; escape.
-  irrelevance0.  1: now rewrite singleSubstComm'.
+  instValid Vσ; instValid Vuσ; escape ; Wescape.
+  unshelve eapply TreeTmEqSplit.
+  1: do 2 eapply DTree_fusion ; [eapply DTree_fusion | eapply DTree_fusion | ..] ; shelve.
+  intros wl'' Ho HA.
+  pose (f':= over_tree_le Ho).
+  Wirrelevance0.  1: now rewrite singleSubstComm'.
   unshelve eapply natElimRedEq; tea; fold subst_term.
-  6-11: irrelevance; now rewrite elimSuccHypTy_subst.
-  3,4: rewrite elimSuccHypTy_subst; eapply validTy; tea; eapply elimSuccHypTyValid.
+  1: econstructor ; eapply  (redtywf_refl (wft_term (ty_nat (wfc_Ltrans f' wfΔ)))).
+  14,15: Wirrelevance0 ; [ now rewrite elimSuccHypTy_subst | now eapply WTm_Ltrans ].
+  14: Wirrelevance0 ; [ now rewrite elimSuccHypTy_subst | now eapply WTmEq_Ltrans ].
+  11,12: Wirrelevance0 ; [ rewrite up_single_subst | now eapply WTm_Ltrans] ; now bsimpl.
+  11: Wirrelevance0 ; [rewrite up_single_subst | now eapply WTmEq_Ltrans] ; now bsimpl.
+  5,6: rewrite elimSuccHypTy_subst; eapply validTy ; [ now eapply elimSuccHypTyValid | ].
+  5,6: now eapply subst_Ltrans.
   + intros m Rm.
     rewrite up_single_subst. 
-    unshelve eapply validTy; cycle 1; tea.
-    unshelve econstructor; [now bsimpl| now cbn].
+    unshelve eapply validTy; cycle 4; tea.
+    1: now eapply wfc_Ltrans.
+    now unshelve econstructor; [eapply subst_Ltrans| eapply TmLogtoW].
+  + irrelevanceRefl.
+    unshelve eapply RVn.
+    1: eapply over_tree_fusion_l, over_tree_fusion_l, over_tree_fusion_l ; exact Ho.
+    eapply over_tree_fusion_r, over_tree_fusion_l, over_tree_fusion_l; exact Ho.
+  + now eapply wfc_Ltrans.
   + intros m Rm.
     rewrite up_single_subst. 
-    unshelve eapply validTy; cycle 1; tea.
-    unshelve econstructor; [now bsimpl| now cbn].
+    unshelve eapply validTy; cycle 4; tea.
+    1: now eapply wfc_Ltrans.
+    now unshelve econstructor; [eapply subst_Ltrans| eapply TmLogtoW].
+  + unshelve eapply validTy; cycle 4; tea.
+    eapply over_tree_fusion_l, over_tree_fusion_r ; exact Ho.
+  + unshelve eapply validTy; cycle 4; tea.
+    eapply over_tree_fusion_r, over_tree_fusion_r ; exact Ho.
+  + now eapply convty_Ltrans.
   + intros m m' Rm Rm' Rmm'; cbn.
-    irrelevance0. 1: now rewrite up_single_subst.
+    Wirrelevance0. 1: now rewrite up_single_subst.
     rewrite up_single_subst.
-    eapply transEq; cycle 1.
-    - unshelve eapply validTyEq. 
-      7: tea. 1: tea.
-      unshelve econstructor; [now bsimpl| now cbn].
-    - unshelve eapply validTyExt; cycle 1 ; tea.
-    1,2: unshelve econstructor; [now bsimpl| now cbn].
-    unshelve econstructor; [|now cbn].
-    bsimpl. eapply reflSubst.
+    eapply WtransEq; cycle 1.
+    * unshelve eapply validTyEq.
+      9: eassumption.
+      1: now eapply wfLCon_le_trans.
+      1: now eapply wfc_Ltrans.
+      now unshelve econstructor; [eapply subst_Ltrans| eapply TmLogtoW].
+    * unshelve eapply validTyExt; cycle 3 ; tea.
+      1: now eapply wfLCon_le_trans.
+      1: now eapply wfc_Ltrans.
+      1,2: now unshelve econstructor; [eapply subst_Ltrans| eapply TmLogtoW].
+      unshelve econstructor; [eapply eqsubst_Ltrans| now eapply TmEqLogtoW].
+      bsimpl. eapply reflSubst.
+  + irrelevance0 ; [ | eapply (WRedTmEq _ RVeqn)].
+    reflexivity.
+    eapply over_tree_fusion_l, over_tree_fusion_r, over_tree_fusion_l ; exact Ho.
+  + irrelevance0 ; [ | eapply (WRedTm _ RVn')].
+    reflexivity.
+    eapply over_tree_fusion_r, over_tree_fusion_r, over_tree_fusion_l ; exact Ho.
+    Unshelve.
+    all: tea.
+    all: now eapply wfc_Ltrans.
 Qed.
 
-Lemma elimSuccHypTyCongValid {Γ l P P'}
-    (VΓ : [||-v Γ])
+Lemma elimSuccHypTyCongValid {wl Γ l P P'}
+    (VΓ : [||-v Γ]< wl >)
     (VN := natValid (l:=l) VΓ)
-    (VΓN := validSnoc VΓ VN)
-    (VP : [Γ ,, tNat ||-v<l> P | VΓN])
-    (VP' : [Γ ,, tNat ||-v<l> P' | VΓN])
-    (VeqP : [Γ ,, tNat ||-v<l> P ≅ P' | VΓN | VP]) :
-    [Γ ||-v<l> elimSuccHypTy P ≅ elimSuccHypTy P' | VΓ | elimSuccHypTyValid VΓ VP].
+    (VΓN := validSnoc' VΓ VN)
+    (VP : [Γ ,, tNat ||-v<l> P | VΓN]< wl >)
+    (VP' : [Γ ,, tNat ||-v<l> P' | VΓN]< wl >)
+    (VeqP : [Γ ,, tNat ||-v<l> P ≅ P' | VΓN | VP]< wl >) :
+    [Γ ||-v<l> elimSuccHypTy P ≅ elimSuccHypTy P' | VΓ | elimSuccHypTyValid VΓ VP]< wl >.
   Proof.
     unfold elimSuccHypTy.
     eapply irrelevanceTyEq.
-    assert [Γ,, tNat ||-v< l > P'[tSucc (tRel 0)]⇑ | validSnoc VΓ VN]. 1:{
+    assert [Γ,, tNat ||-v< l > P'[tSucc (tRel 0)]⇑ | validSnoc' VΓ VN]< wl >. 1:{
       eapply substLiftS; tea.
       eapply irrelevanceTm.
       eapply succValid.
